theories/dfs_xleroy/README.md
@@ -2,7 +2,7 @@
 
 ## Introduction
 
-The motivation for this study is the CoqPL 2024 paper _[Well founded recursion done right](https://popl24.sigplan.org/details/CoqPL-2024-papers/2/Well-founded-recursion-done-right) by Xavier Leroy_, which elaborates on a Depth First Search algorithm (DFS) in its appendix B, called `dfs_xl` herein. Although this algorithm is explicitly dedicated to direct acyclic graphs (DAGs), it is easy to see how a slight change in a single line (of the intended extracted code) of `dfs_xl` allows one to recover a DFS without restriction (called `dfs_cycle` herein).
+The motivation for this study is the CoqPL 2024 paper _[Well founded recursion done right](https://popl24.sigplan.org/details/CoqPL-2024-papers/2/Well-founded-recursion-done-right) by Xavier Leroy_, which elaborates on a Depth First Search algorithm (DFS) in its appendix B, called `dfs_xl` herein. Although this algorithm is explicitly dedicated to direct acyclic graphs (DAGs), it is easy to see how a slight mutation in a single line (of the intended extracted code) of `dfs_xl` allows one to recover a DFS without restriction (called `dfs_cycle` herein).
 
 In the [_Braga method book chapter_](https://www.worldscientific.com/doi/abs/10.1142/9789811236488_0008) (see also the [Braga method on GitHub](https://github.com/DmxLarchey/The-Braga-Method/)), we extensively studied another DFS algorithm simply called `dfs` there but herein called `dfs_book` for disambiguation.
 
@@ -11,7 +11,7 @@ It was thus natural for us to (and we felt compelled to):
 - compare the semantics of `dfs_xl` and `dfs_book`:
   + ie. their respective domains of termination;
   + and the respective specifications of their output;
-- instantiate the Braga method on `dfs_cycle`  as well (the slightly modified variant of `dfs_xl`) and study its relationship with `dfs_book`; the latter turns out to be retrieved step by step from `dfs_cycle` using simple transformations, but the semantic equivalence can also be justified using tools developed for the Braga method.
+- instantiate the Braga method on `dfs_cycle` as well (the slightly modified variant of `dfs_xl`) and study its relationship with `dfs_book`; the latter turns out to be retrieved step by step from `dfs_cycle` using simple transformations, but the semantic equivalence can also be justified using tools developed for the Braga method.
  
 Notice that general DFS algorithms are inherently partial algorithms:
 - when the type of vertices is infinite, there can be a cycle-free infinite path in the graph;
@@ -32,7 +32,7 @@ succs : 𝓥 -> 𝓥 list
 where `𝓥` is a type of vertices, `succs` describes a finitely branching directed graph structure (but not necessarily finite or acyclic though), and `∈` is a membership test for lists, abstracted of the specificities of its implementation, and denoted with an infix notation.
 
 We will also sometimes need the following polymorphic implementation of the higher-order function `foldleft`
-```
+```ocaml
 (* foldleft : (β -> α -> α) -> β list -> α -> α *)
 let rec foldleft f l a = match l with
 | []   -> a
@@ -45,7 +45,7 @@ which only differs from the Ocaml one `List.fold_left` in the order of parameter
 ### The nested algorithm `dfs_xl`
 
 Given these assumptions, the algorithm studied by X. Leroy in CoqPL 2024 could be described as the following Ocaml program. Notice that _only its Coq enrichment is actually written in the paper_:
-```
+```ocaml
 (* DFS variant by X. Leroy as in CoqPL'2024 *)
 let dfs_xl_inld x =
   let rec dfs x a =
@@ -84,7 +84,7 @@ One could wonder why X. Leroy did not favor this external nesting (more compact,
 Another observation that could be made regarding `dfs_xl` is the position where `x` is prepended to the already visited nodes using `x::_`. In `dfs_xl` this occurs after the successors of `x` are visited by `foldleft dfs (succs x) a`, hence we speculate that when `dfs` visits a node contained in a cycle, the algorithm will loop forever. We will indeed prove that `dfs_xl` is for DAGs only. 
  
 A slight change provides a version of DFS which will avoid this behavior and which we call `dfs_cycle`. The easiest way to observe the change is on the externally nested variant:
-```
+```ocaml
 (* DFS variant of dfs_xl_fold which accommodates with cycles *)
 let dfs_cycle_fold x =
   let rec dfs x a =
@@ -92,7 +92,7 @@ let dfs_cycle_fold x =
   in dfs x []
 ```
 but the inlined nested variant works just as well:
-```
+```ocaml
 (* Variant of dfs_cycle with inlined nesting *)
 let dfs_cycle_inld x =
   let rec dfs x a =
@@ -107,7 +107,7 @@ let dfs_cycle_inld x =
 ### The recursive terminal algorithm `dfs_book`
 
 In the Braga book chapter however, we study the following variant of DFS
-```
+```ocaml
 (* DFS variant as described in the Braga book chapter *)
 let dfs_book x =
   let rec dfs a = function
@@ -118,7 +118,9 @@ let dfs_book x =
 that uses list append/`@` as an external tool (of linear complexity). Notice that the internal loop `dfs` in `dfs_book` is _not a nested algorithm_ and it is moreover a recursive terminal algorithm. Also, the accumulator `a` which collects already visited nodes in the internal `dfs` appears first in `dfs_book` whereas it appears last for `dfs_xl` and `dfs_cycle`.
 
 _JFM->DLW : arrivé ici je me rends compte que sauf erreur de ma part on parle de `dfs_cycle`, sous la forme avec foldleft. Il me paraît plus judicieux d'introduire soit cette variante `_fold`, soit  celle "nested" inspirée de XL dès le début `_inld`, comme ce que j'ai ajouté. Pour l'instant je laisse ce qui suit, mais peut-être que la suite plus bas pourra être allégée. Mes transfos partent de `dfs_cycle_inld` mais comme on dérive plus facilement ce dernier de `dfs_cycle_fold` (par dépliage de foldleft) que l'inverse, on peut prendre `dfs_cycle_fold`  comme pt de départ. Et du coup je remonter le code de `dfs_braga_cycle` plus haut._
-_DLW->JFM: c'est fait j'ai remonté `dfs_braga` et maintenant renommé `dfs_cycle_fold`. Je préfère que tu partes de celui-là pour tes transformations car il me semble plus facile d'expliquer la différence avec `dfs_xl_fold`._
+_DLW->JFM: c'est fait j'ai remonté `dfs_braga` et maintenant renommé `dfs_cycle_fold`. Je préfère que tu partes de celui-là pour tes transformations car il me semble plus facile d'expliquer la différence avec `dfs_xl_fold`.
+JFL->DLW: d'ac pour partir dans le README de `dfs_cycle_fold` car c'est plus compact
+et trivialement dérivable seult dans cette direction; mais la différence est la même._
 
 It is not immediate that `dfs_book` and `dfs_cycle` compute the same thing which means that they both have the same domain of termination and output exactly the same list, but we mechanise this proof and show their equivalence.
 
@@ -130,6 +132,10 @@ If we compare the respective codes of the most compact variants `dfs_xl_fold` an
 - in `dfs_xl_fold    : ... x::(foldleft dfs (succs x) a) ...`;
 - in `dfs_cycle_fold : ... foldleft dfs (succs x) (x::a) ...`.
 
+Of course, the same mutation operates on the variants expressed with nested recursion:
+- in `dfs_xl_inld    : ... x::(dfs_list (succs x) a) ...`;
+- in `dfs_cycle_inld : ... dfs_list (succs x) (x::a) ...`.
+
 This change has a significant impact on the semantics:
 - on the order of the output list of course,
 - but mainly the weakest precondition for termination (wrt. cycles in the graph).
@@ -140,15 +146,16 @@ _JFM->DLW : il faut revoir la fin en fonction des modifs précédentes , pour in
 _JFM->DLW : finalement j'ai intégré ma partie, j'espère que c'est compatible avec ce que tu voulais._
 
 To complete our exploration, we also study the following variants of `dfs_xl` with _self-nesting_ of its internal loop `dfs`:
-```
+```ocaml
 let dfs_xl_self x =
   let rec dfs_list l a = match l with 
   | []   -> a
   | x::l -> dfs_list l (if x ∈ a then a else x::dfs_list (succs x) a)
   in dfs_list [x] []
 ```
-Interestingly, the self nested variant `dfs_cycle_self` is the first step towards a variant of  `dfs_book` avoiding the use of the external append/`@` and then `dfs_book` itself. _DLW->JFM: préciser le sens ici..._
-```
+Interestingly, the self nested variant `dfs_cycle_self` is the first step towards a variant of  `dfs_book` called `dfs_book_eff` (it is somewhat more efficient since its avoids computating the concatenation of lists) and then `dfs_book` itself. _DLW->JFM: préciser le sens ici...
+JFM->DLW: le sens de ? En tout cas j'ai renommé `dfs_cycle_grp` qui n'était pas très heureux_
+```ocaml
 let dfs_cycle_self x =
   let rec dfs_list a = function
   | []   -> a
@@ -156,20 +163,20 @@ let dfs_cycle_self x =
   in dfs_list [x] []
 ```
 In the second step, the (implicit) stack of recursive calls is implemented using an explicit stack of lists `s`; in particular nested recursive calls are eliminated.
-```
+```ocaml
 let dfs_cycle_stack x =
-  let rec dfs_stack a = function
+  let rec dfs_list_stack a = function
   | []   -> (function
     | []   -> a
-    | l::s -> dfs_stack a l s)
+    | l::s -> dfs_list_stack a l s)
   | x::l -> fun s ->
-    if x ∈ a then dfs_stack a l s
-    else dfs_stack (x::a) (succs x) (l::s) 
-  in dfs_stack [] [x] []
+    if x ∈ a then dfs_list_stack a l s
+    else dfs_list_stack (x::a) (succs x) (l::s) 
+  in dfs_list_stack [] [x] []
 ```
 Next step: `l` and `s` are grouped into a single list of lists `ls` which represents `l::s`:
-```
-let dfs_cycle_grp x =
+```ocaml
+let dfs_book_eff x =
   let rec dfs_stack a = function
   | []         -> a
   | []::ls     -> dfs_stack a ls
@@ -179,6 +186,16 @@ let dfs_cycle_grp x =
   in dfs_stack [] [[x]]
 ```
 Finally `dfs_book` is obtained by flattening `ls`, so that `(x::l)::ls`is represented by `x::lls` and `succs x::l::ls` is represented by `succs x @ lls` and `lls` is renamed as just `l`.
+Next step: `l` and `s` are grouped into a single list of lists `ls` which represents `l::s`:
+```ocaml
+let dfs_book x =
+  let rec dfs_flatten a = function
+  | []         -> a
+  | x::lls ->
+    if x ∈ a then dfs_flatten a lls
+    else dfs_flatten (x::a) (succs x::lls) 
+  in dfs_flatten [] [x]
+```
 
 
 
